add an  Nat to all typedefs using Nat

CompositionalProtocolProof/EventRelations.lean
@@ -1,25 +1,27 @@
 import CompositionalProtocolProof.Events
 import CompositionalProtocolProof.Requests
 
-def Event.Encapsulates (e₁ e₂ : Event) : Prop := e₁.oStart < e₂.oStart ∧ e₂.oEnd < e₁.oEnd
-def CacheEvent.Encapsulates (e₁ e₂ : CacheEvent) : Prop := e₁.oStart < e₂.oStart ∧ e₂.oEnd < e₁.oEnd
-def DirectoryEvent.Encapsulates (e₁ e₂ : DirectoryEvent) : Prop := e₁.oStart < e₂.oStart ∧ e₂.oEnd < e₁.oEnd
+variable (n : Nat)
 
-def Event.OrderedBefore (e₁ e₂ : Event) : Prop := e₁.oEnd < e₂.oStart
-def CacheEvent.OrderedBefore (e₁ e₂ : CacheEvent) : Prop := e₁.oEnd < e₂.oStart
-def DirectoryEvent.OrderedBefore (e₁ e₂ : DirectoryEvent) : Prop := e₁.oEnd < e₂.oStart
+def Event.Encapsulates (e₁ e₂ : Event n) : Prop := e₁.oStart < e₂.oStart ∧ e₂.oEnd < e₁.oEnd
+def CacheEvent.Encapsulates (e₁ e₂ : CacheEvent n) : Prop := e₁.oStart < e₂.oStart ∧ e₂.oEnd < e₁.oEnd
+def DirectoryEvent.Encapsulates (e₁ e₂ : DirectoryEvent n) : Prop := e₁.oStart < e₂.oStart ∧ e₂.oEnd < e₁.oEnd
 
-def Event.Ordered (e₁ e₂ : Event) : Prop := e₁.OrderedBefore e₂ ∨ e₂.OrderedBefore e₁
-def CacheEvent.Ordered (e₁ e₂ : CacheEvent) : Prop := e₁.OrderedBefore e₂ ∨ e₂.OrderedBefore e₁
-def DirectoryEvent.Ordered (e₁ e₂ : DirectoryEvent) : Prop := e₁.OrderedBefore e₂ ∨ e₂.OrderedBefore e₁
+def Event.OrderedBefore (e₁ e₂ : Event n) : Prop := e₁.oEnd < e₂.oStart
+def CacheEvent.OrderedBefore (e₁ e₂ : CacheEvent n) : Prop := e₁.oEnd < e₂.oStart
+def DirectoryEvent.OrderedBefore (e₁ e₂ : DirectoryEvent n) : Prop := e₁.oEnd < e₂.oStart
 
-def Event.fromDirectoryEvent (de : DirectoryEvent) (e : Event) : Prop :=
+def Event.Ordered (e₁ e₂ : Event n) : Prop := e₁.OrderedBefore n e₂ ∨ e₂.OrderedBefore n e₁
+def CacheEvent.Ordered (e₁ e₂ : CacheEvent n) : Prop := e₁.OrderedBefore n e₂ ∨ e₂.OrderedBefore n e₁
+def DirectoryEvent.Ordered (e₁ e₂ : DirectoryEvent n) : Prop := e₁.OrderedBefore n e₂ ∨ e₂.OrderedBefore n e₁
+
+def Event.fromDirectoryEvent (de : DirectoryEvent n) (e : Event n) : Prop :=
   match e with
   | .directoryEvent de' => de = de'
   | .cacheEvent _ => false
 
-lemma DirectoryEvent.ordered_events {de₁ de₂ : DirectoryEvent} {e₁ e₂ : Event}
-  (he₁_is_de₁ : e₁.fromDirectoryEvent de₁) (he₂_is_de₂ : e₂.fromDirectoryEvent de₂) : de₁.OrderedBefore de₂ → e₁.OrderedBefore e₂ := by
+lemma DirectoryEvent.ordered_events {de₁ de₂ : DirectoryEvent n} {e₁ e₂ : Event n}
+  (he₁_is_de₁ : e₁.fromDirectoryEvent n de₁) (he₂_is_de₂ : e₂.fromDirectoryEvent n de₂) : de₁.OrderedBefore n de₂ → e₁.OrderedBefore n e₂ := by
   unfold DirectoryEvent.OrderedBefore; unfold Event.OrderedBefore
   -- unfold DirectoryEvent.oEnd; unfold DirectoryEvent.oStart
   unfold Event.oEnd; unfold Event.oStart
@@ -33,27 +35,27 @@ lemma DirectoryEvent.ordered_events {de₁ de₂ : DirectoryEvent} {e₁ e₂ : 
   | .cacheEvent _, .directoryEvent _ => contradiction
   | .cacheEvent _, .cacheEvent _ => contradiction
 
-def Event.Predecessor : Event → Event → Prop
-| e_pred, e_succ => e_pred.OrderedBefore e_succ
+def Event.Predecessor : Event n → Event n → Prop
+| e_pred, e_succ => e_pred.OrderedBefore n e_succ
 
-def Event.Successor : Event → Event → Prop
-| e_pred, e_succ => e_pred.Predecessor e_succ
+def Event.Successor : Event n → Event n → Prop
+| e_pred, e_succ => e_pred.Predecessor n e_succ
 
-instance Event.Encapsulates.instDecidableEncap (e₁ e₂ : Event) : Decidable (e₁.Encapsulates e₂) :=
+instance Event.Encapsulates.instDecidableEncap (e₁ e₂ : Event n) : Decidable (e₁.Encapsulates n e₂) :=
   inferInstanceAs (Decidable (e₁.oStart < e₂.oStart ∧ e₂.oEnd < e₁.oEnd))
 
-instance Event.OrderedBefore.instLT : LT Event := {lt := Event.OrderedBefore}
+instance Event.OrderedBefore.instLT : LT (Event n) := {lt := Event.OrderedBefore n}
 
-instance Event.OrderedBefore.instDecidableLT (e₁ e₂ : Event) : Decidable (e₁ < e₂) :=
+instance Event.OrderedBefore.instDecidableLT (e₁ e₂ : Event n) : Decidable (e₁ < e₂) :=
   inferInstanceAs (Decidable (e₁.oEnd < e₂.oStart))
 
-instance Event.OrderedBefore.instDecidableRel : DecidableRel Event.OrderedBefore := by
+instance Event.OrderedBefore.instDecidableRel : DecidableRel (Event.OrderedBefore n) := by
   unfold DecidableRel
   intro e₁ e₂
   unfold Event.OrderedBefore
   infer_instance
 
-lemma Event.ordered_trans {e₁ e₂ e₃ : Event} : e₁ < e₂ → e₂ < e₃ → e₁ < e₃ := by
+lemma Event.ordered_trans {e₁ e₂ e₃ : Event n} : e₁ < e₂ → e₂ < e₃ → e₁ < e₃ := by
   unfold LT.lt; unfold OrderedBefore.instLT
   simp
   unfold Event.OrderedBefore;
@@ -64,9 +66,9 @@ lemma Event.ordered_trans {e₁ e₂ e₃ : Event} : e₁ < e₂ → e₂ < e₃
     _ < e₂.oEnd := he₂_well_formed
     _ < e₃.oStart := he₂_lt_e₃
 
-instance Event.instTransOrderOrder : Trans Event.OrderedBefore Event.OrderedBefore Event.OrderedBefore := {trans := Event.ordered_trans}
+instance Event.instTransOrderOrder : Trans (Event.OrderedBefore n) (Event.OrderedBefore n) (Event.OrderedBefore n) := {trans := Event.ordered_trans n}
 
-lemma Event.order_encap_trans {e₁ e₂ e₃ : Event} : e₁ < e₂ → e₂.Encapsulates e₃ → e₁ < e₃ := by
+lemma Event.order_encap_trans {e₁ e₂ e₃ : Event n} : e₁ < e₂ → e₂.Encapsulates n e₃ → e₁ < e₃ := by
   unfold LT.lt; unfold OrderedBefore.instLT
   simp
   unfold Event.OrderedBefore;
@@ -76,11 +78,11 @@ lemma Event.order_encap_trans {e₁ e₂ e₃ : Event} : e₁ < e₂ → e₂.En
     e₁.oEnd < e₂.oStart := he₁_lt_e₂
     _ < e₃.oStart := he₂_encap_e₃.left
 
-instance Event.instTransOrderEncap : Trans Event.OrderedBefore Event.Encapsulates Event.OrderedBefore := {trans := Event.order_encap_trans}
+instance Event.instTransOrderEncap : Trans (Event.OrderedBefore n) (Event.Encapsulates n) (Event.OrderedBefore n) := {trans := Event.order_encap_trans n}
 
-abbrev Event.EncapsulatedBy (e₁ e₂ : Event) : Prop := e₂.Encapsulates e₁
+abbrev Event.EncapsulatedBy (e₁ e₂ : Event n) : Prop := e₂.Encapsulates n e₁
 
-lemma Event.encap_by_order_trans {e₁ e₂ e₃ : Event} : e₁.EncapsulatedBy e₂ → e₂ < e₃ → e₁ < e₃ := by
+lemma Event.encap_by_order_trans {e₁ e₂ e₃ : Event n} : e₁.EncapsulatedBy n e₂ → e₂ < e₃ → e₁ < e₃ := by
   unfold LT.lt; unfold OrderedBefore.instLT
   simp
   -- unfold BottomEncapsulates;
@@ -93,17 +95,17 @@ lemma Event.encap_by_order_trans {e₁ e₂ e₃ : Event} : e₁.EncapsulatedBy 
     _ < e₃.oStart := he₂_lt_e₃
 
 /- The shape of Trans's definition doesn't match to Event.encap_order_trans. Need to massage def. -/
-instance Event.instTransEncapByOrder : Trans Event.EncapsulatedBy Event.OrderedBefore Event.OrderedBefore := {trans := Event.encap_by_order_trans}
+instance Event.instTransEncapByOrder : Trans (Event.EncapsulatedBy n) (Event.OrderedBefore n) (Event.OrderedBefore n) := {trans := Event.encap_by_order_trans n}
 
-structure Event.OrderedBetween (e e_pred e_succ : Event) where
-  pred : e_pred.OrderedBefore e := by simp
-  succ : e.OrderedBefore e_succ := by simp
+structure Event.OrderedBetween (e e_pred e_succ : Event n) where
+  pred : e_pred.OrderedBefore n e := by simp
+  succ : e.OrderedBefore n e_succ := by simp
 
-def CacheEvent.SameRequester (e₁ e₂ : CacheEvent) : Prop := e₁.rid = e₂.rid
-def CacheEvent.SameCache (e₁ e₂ : CacheEvent) : Prop := e₁.cid = e₂.cid
-def CacheEvent.SameAddress (e₁ e₂ : CacheEvent) : Prop := e₁.addr = e₂.addr
+def CacheEvent.SameRequester (e₁ e₂ : CacheEvent n) : Prop := e₁.rid = e₂.rid
+def CacheEvent.SameCache (e₁ e₂ : CacheEvent n) : Prop := e₁.cid = e₂.cid
+def CacheEvent.SameAddress (e₁ e₂ : CacheEvent n) : Prop := e₁.addr = e₂.addr
 
-def Event.CacheRelation (e₁ e₂ : Event) : (CacheEvent → CacheEvent → Prop) → Prop
+def Event.CacheRelation (e₁ e₂ : Event n) : (CacheEvent n → CacheEvent n → Prop) → Prop
 | p => match e₁ with
   | .cacheEvent ce₁ =>
     match e₂ with
@@ -111,8 +113,8 @@ def Event.CacheRelation (e₁ e₂ : Event) : (CacheEvent → CacheEvent → Pro
     | .directoryEvent _ => false -- nothing happens
   | .directoryEvent _ => false -- nothing happens
 
-def Event.SameStructureRelation (e₁ e₂ : Event) :
-  (CacheEvent → CacheEvent → Prop) → (DirectoryEvent → DirectoryEvent → Prop) → Prop
+def Event.SameStructureRelation (e₁ e₂ : Event n) :
+  (CacheEvent n → CacheEvent n → Prop) → (DirectoryEvent n → DirectoryEvent n → Prop) → Prop
 | cp, dp => match e₁ with
   | .cacheEvent ce₁ =>
     match e₂ with
@@ -124,14 +126,14 @@ def Event.SameStructureRelation (e₁ e₂ : Event) :
     | .directoryEvent de₂ => dp de₁ de₂
 
 -- abbrev CacheEvent.SameRequester (e₁ e₂ : CacheEvent) : Prop := e₁.rid = e₂.rid
-def DirectoryEvent.SameStructure (_ _ : DirectoryEvent) : Prop := true
-def DirectoryEvent.SameAddress (e₁ e₂ : DirectoryEvent) : Prop := e₁.addr = e₂.addr
+def DirectoryEvent.SameStructure (_ _ : DirectoryEvent n) : Prop := true
+def DirectoryEvent.SameAddress (e₁ e₂ : DirectoryEvent n) : Prop := e₁.addr = e₂.addr
 
-def Event.CacheSameRequester (e₁ e₂ : Event) : Prop := e₁.CacheRelation e₂ (·.SameRequester ·)
-def Event.SameStructure (e₁ e₂ : Event) : Prop := e₁.SameStructureRelation e₂ (·.SameCache ·) (·.SameStructure ·)
-def Event.SameAddress (e₁ e₂ : Event) : Prop := e₁.SameStructureRelation e₂ (·.SameAddress ·) (·.SameAddress ·)
+def Event.CacheSameRequester (e₁ e₂ : Event n) : Prop := e₁.CacheRelation n e₂ (·.SameRequester n ·)
+def Event.SameStructure (e₁ e₂ : Event n) : Prop := e₁.SameStructureRelation n e₂ (·.SameCache n ·) (·.SameStructure n ·)
+def Event.SameAddress (e₁ e₂ : Event n) : Prop := e₁.SameStructureRelation n e₂ (·.SameAddress n ·) (·.SameAddress n ·)
 
-lemma Event.same_address_reflexive {e₁ e₂ e₃ : Event} : e₁.SameAddress e₃ → e₂.SameAddress e₃ → e₁.SameAddress e₂ := by
+lemma Event.same_address_reflexive {e₁ e₂ e₃ : Event n} : e₁.SameAddress n e₃ → e₂.SameAddress n e₃ → e₁.SameAddress n e₂ := by
   unfold SameAddress
   unfold CacheEvent.SameAddress; unfold DirectoryEvent.SameAddress
   unfold SameStructureRelation
@@ -147,7 +149,7 @@ lemma Event.same_address_reflexive {e₁ e₂ e₃ : Event} : e₁.SameAddress e
   | .directoryEvent de₁, .cacheEvent ce, .directoryEvent de₃ => contradiction
   | .cacheEvent ce, .directoryEvent de₂, .directoryEvent de₃ => contradiction
 
-lemma Event.same_address_reflexive' {e₁ e₂ e₃ : Event} : e₁.SameAddress e₂ → e₁.SameAddress e₃ → e₂.SameAddress e₃ := by
+lemma Event.same_address_reflexive' {e₁ e₂ e₃ : Event n} : e₁.SameAddress n e₂ → e₁.SameAddress n e₃ → e₂.SameAddress n e₃ := by
   unfold SameAddress
   unfold CacheEvent.SameAddress; unfold DirectoryEvent.SameAddress
   unfold SameStructureRelation
@@ -163,7 +165,7 @@ lemma Event.same_address_reflexive' {e₁ e₂ e₃ : Event} : e₁.SameAddress 
   | .directoryEvent de₁, .cacheEvent ce, .directoryEvent de₃ => contradiction
   | .cacheEvent ce, .directoryEvent de₂, .directoryEvent de₃ => contradiction
 
-lemma Event.same_structure_reflexive {e₁ e₂ e₃ : Event} : e₁.SameStructure e₃ → e₂.SameStructure e₃ → e₁.SameStructure e₂ := by
+lemma Event.same_structure_reflexive {e₁ e₂ e₃ : Event n} : e₁.SameStructure n e₃ → e₂.SameStructure n e₃ → e₁.SameStructure n e₂ := by
   unfold SameStructure
   unfold CacheEvent.SameCache; unfold DirectoryEvent.SameStructure
   unfold SameStructureRelation
@@ -179,7 +181,7 @@ lemma Event.same_structure_reflexive {e₁ e₂ e₃ : Event} : e₁.SameStructu
   | .directoryEvent de₁, .cacheEvent ce, .directoryEvent de₃ => contradiction
   | .cacheEvent ce, .directoryEvent de₂, .directoryEvent de₃ => contradiction
 
-lemma Event.same_structure_reflexive' {e₁ e₂ e₃ : Event} : e₁.SameStructure e₂ → e₁.SameStructure e₃ → e₂.SameStructure e₃ := by
+lemma Event.same_structure_reflexive' {e₁ e₂ e₃ : Event n} : e₁.SameStructure n e₂ → e₁.SameStructure n e₃ → e₂.SameStructure n e₃ := by
   unfold SameStructure
   unfold CacheEvent.SameCache; unfold DirectoryEvent.SameStructure
   unfold SameStructureRelation
@@ -195,18 +197,18 @@ lemma Event.same_structure_reflexive' {e₁ e₂ e₃ : Event} : e₁.SameStruct
   | .directoryEvent de₁, .cacheEvent ce, .directoryEvent de₃ => contradiction
   | .cacheEvent ce, .directoryEvent de₂, .directoryEvent de₃ => contradiction
 
-structure CacheEvent.ProgramOrdered (e₁ e₂ : CacheEvent) where
-  ordered : e₁.OrderedBefore e₂ := by simp
-  same_requester : e₁.SameRequester e₂ := by simp
+structure CacheEvent.ProgramOrdered (e₁ e₂ : CacheEvent n) where
+  ordered : e₁.OrderedBefore n e₂ := by simp
+  same_requester : e₁.SameRequester n e₂ := by simp
 
-def Event.ProgramOrdered (e₁ e₂ : Event) : Prop := e₁.CacheRelation e₂ (·.ProgramOrdered ·)
+def Event.ProgramOrdered (e₁ e₂ : Event n) : Prop := e₁.CacheRelation n e₂ (·.ProgramOrdered n ·)
 
 /-- Axiom 1
 Events at a Directory address are ordered.
 -/
-structure DirectoryEvent.AreOrdered (de₁ de₂ : DirectoryEvent) : Prop where
+structure DirectoryEvent.AreOrdered (de₁ de₂ : DirectoryEvent n) : Prop where
   sameDirectoryEntry : de₁.addr = de₂.addr
-  ordered : de₁.Ordered de₂
+  ordered : de₁.Ordered n de₂
 /-
 def Event.isDirectoryEvent : Event → Prop
 | .directoryEvent _ => true
@@ -218,52 +220,52 @@ def OrderedDirectoryEvents' (e₁ e₂ : Event) : Prop :=
 /-- Definition 2.18. Directory Event ID.
 Ordered Directory Events.
 -/
-def MonotonicDirectoryEventIds (de₁ de₂ : DirectoryEvent) : Prop := de₁.OrderedBefore de₂ → (de₁.deid + 1) = de₂.deid
+def MonotonicDirectoryEventIds (de₁ de₂ : DirectoryEvent n) : Prop := de₁.OrderedBefore n de₂ → (de₁.deid + 1) = de₂.deid
 
 /- Lean can't synthesize decidability in OrderedCacheEvents if these aren't `abbrev`s -/
-abbrev CacheEvent.Local (e : CacheEvent) : Prop := e.cid = e.rid
-abbrev CacheEvent.NonCoherent (e : CacheEvent) : Prop := e.req.val.coherent = false
-abbrev CacheEvent.WeakConsistency (e : CacheEvent) : Prop := e.req.val.consistency = .Weak
+abbrev CacheEvent.Local (e : CacheEvent n) : Prop := e.cid = e.rid
+abbrev CacheEvent.NonCoherent (e : CacheEvent n) : Prop := e.req.val.coherent = false
+abbrev CacheEvent.WeakConsistency (e : CacheEvent n) : Prop := e.req.val.consistency = .Weak
 
-abbrev CacheEvent.Weak (e : CacheEvent) : Prop := e.Local ∧ e.NonCoherent ∧ e.WeakConsistency
+abbrev CacheEvent.Weak (e : CacheEvent n) : Prop := e.Local ∧ e.NonCoherent ∧ e.WeakConsistency
 
-abbrev CacheEvent.RequestHasPermissions (e : CacheEvent) (s : State) : Prop := e.req.MRS ≤ s
-abbrev CacheEvent.Coherent (e : CacheEvent) : Prop := e.req.val.coherent = true
+abbrev CacheEvent.RequestHasPermissions (e : CacheEvent n) (s : State) : Prop := e.req.MRS ≤ s
+abbrev CacheEvent.Coherent (e : CacheEvent n) : Prop := e.req.val.coherent = true
 
-abbrev CacheEvent.WithCoherentPermissions (e : CacheEvent) (s : State) : Prop := e.Local ∧ e.Coherent ∧ e.RequestHasPermissions s
+abbrev CacheEvent.WithCoherentPermissions (e : CacheEvent n) (s : State) : Prop := e.Local ∧ e.Coherent ∧ e.RequestHasPermissions n s
 
-abbrev CacheEvent.Downgrade (e : CacheEvent) : Prop := e.down = true
-abbrev CacheEvent.NoEncapSameAddressDowngrade (e : CacheEvent) (s : State) : Prop := e.Weak ∨ e.WithCoherentPermissions s ∨ e.Downgrade
+abbrev CacheEvent.Downgrade (e : CacheEvent n) : Prop := e.down = true
+abbrev CacheEvent.NoEncapSameAddressDowngrade (e : CacheEvent n) (s : State) : Prop := e.Weak ∨ e.WithCoherentPermissions n s ∨ e.Downgrade
 
-abbrev CacheEvent.Grant (e : CacheEvent) : Prop := e.deid? ≠ none
-abbrev CacheEvent.External (e : CacheEvent) : Prop := ¬e.Local ∨ e.Grant
-abbrev CacheEvent.NoRequestPermissions (e : CacheEvent) (s : State) : Prop := s < e.req.MRS ∧ s ≠ I
+abbrev CacheEvent.Grant (e : CacheEvent n) : Prop := e.deid? ≠ none
+abbrev CacheEvent.External (e : CacheEvent n) : Prop := ¬e.Local ∨ e.Grant
+abbrev CacheEvent.NoRequestPermissions (e : CacheEvent n) (s : State) : Prop := s < e.req.MRS ∧ s ≠ I
 
-abbrev CacheEvent.WithoutCoherentPermissions (e : CacheEvent) (s : State) : Prop := e.Local ∧ e.Coherent ∧ e.NoRequestPermissions s
+abbrev CacheEvent.WithoutCoherentPermissions (e : CacheEvent n) (s : State) : Prop := e.Local ∧ e.Coherent ∧ e.NoRequestPermissions n s
 
-structure CacheEvent.sameCacheEntry (e₁ e₂ : CacheEvent) : Prop where
+structure CacheEvent.sameCacheEntry (e₁ e₂ : CacheEvent n) : Prop where
   sameCache : e₁.cid = e₂.cid
   sameAddr : e₁.addr = e₂.addr
 
-structure Event.sameStructure (e₁ e₂ : Event) : Prop where
+structure Event.sameStructure (e₁ e₂ : Event n) : Prop where
   sameStruct : e₁.struct = e₂.struct
 
-structure Event.sameAddr (e₁ e₂ : Event) : Prop where
+structure Event.sameAddr (e₁ e₂ : Event n) : Prop where
   sameStruct : e₁.addr = e₂.addr
 
 structure Event.sameEntry : Prop where
-  sameStruct : ∀ e₁ e₂ : Event, e₁.sameStructure e₂
-  sameAddr : ∀ e₁ e₂ : Event, e₁.sameAddr e₂
+  sameStruct : ∀ e₁ e₂ : Event n, e₁.sameStructure n e₂
+  sameAddr : ∀ e₁ e₂ : Event n, e₁.sameAddr n e₂
 
 def CoherentRead : Request := ⟨ .r, true, .SC ⟩
 def CoherentWrite : Request := ⟨ .w, true, .SC ⟩
 
-def CacheEvent.SucceedingState (e : CacheEvent) (s : State) : State :=
+def CacheEvent.SucceedingState (e : CacheEvent n) (s : State) : State :=
   match e.down with
   | false => e.req.RequestState s
   | true => e.req.DowngradeState s
 
-def DirectoryEvent.SucceedingState : /- ProtocolInterface → -/ DirectoryEvent → DirectoryState → DirectoryState
+def DirectoryEvent.SucceedingState : /- ProtocolInterface → -/ DirectoryEvent n → DirectoryState n → DirectoryState n
 | de, ds => match de.down with
   | false => match de.req.val with
     | ⟨.w, true, _⟩ => -- Coherent-Write
@@ -300,22 +302,22 @@ def DirectoryEvent.SucceedingState : /- ProtocolInterface → -/ DirectoryEvent 
    OR build in the input state and interface requests into the types.
 -/
 
-def Event.SucceedingState (e : Event) (s : EntryState) : EntryState := match e with
-  | .cacheEvent ce => ⟨ce.SucceedingState s.cache, s.directory⟩
-  | .directoryEvent de => ⟨s.cache, de.SucceedingState s.directory⟩
+def Event.SucceedingState (e : Event n) (s : EntryState n) : EntryState n := match e with
+  | .cacheEvent ce => ⟨ce.SucceedingState n s.cache, s.directory⟩
+  | .directoryEvent de => ⟨s.cache, de.SucceedingState n s.directory⟩
 
-structure Event.fwdRequest (e_req e_fwd : Event) : Prop where
+structure Event.fwdRequest (e_req e_fwd : Event n) : Prop where
   sameRequest : e_req.req = e_fwd.req
-  sameRequester : e_req.CacheSameRequester e_fwd
-  sameAddr : e_req.sameAddr e_fwd
+  sameRequester : e_req.CacheSameRequester n e_fwd
+  sameAddr : e_req.sameAddr n e_fwd
 
 /-- Definition 2.35 -- A Downgrade Event generated by a corresponding to a Request Event -/
 structure Event.downgradeOfRequestToOthers : Prop where
-  atCid   : ∀ e_down : Event, ∀ cid : CacheId, e_down.isCacheEventAtCid cid
-  isDown  : ∀ e_down : Event, e_down.isCacheEventDowngrade
-  isFwded : ∀ e_req e_down : Event, e_req.fwdRequest e_down
+  atCid   : ∀ e_down : Event n, ∀ cid : CacheId n, e_down.isCacheEventAtCid n cid
+  isDown  : ∀ e_down : Event n, e_down.isCacheEventDowngrade
+  isFwded : ∀ e_req e_down : Event n, e_req.fwdRequest n e_down
 
-def Event.isDirEventOfReqEvent : Event → Event → Prop
+def Event.isDirEventOfReqEvent : Event n → Event n → Prop
 | e_dir, e_req => match e_dir with
   | .directoryEvent de => match e_req with
     | .cacheEvent ce => de.eReq = ce
